\documentclass[12pt]{report}
\usepackage{amsmath}
\usepackage{graphicx}
\begin{document}
boost


Basic Equations
\begin{align}
I_{ref}(\theta) = \frac{P_{o}}{V_{pk}}\\
\delta_{Q}(\theta) = 1 - \frac{V_{pk}}{V_{o}}\\
\delta_{D}(\theta) = \frac{V_{pk}}{V_{o}}\\
\end{align}

Bilateral Triangle $\Delta^B$ 

A = triangle peak-to-peak 

DT = time of triangle peak
\begin{align}
\Delta^B_{rms}(A,B,D,T) = \frac{\sqrt{\int\limits_{0}^{D T} \left(- \frac{A}{2} + \frac{A t}{D T}\right)^{2}\, dt + \int\limits_{0}^{T \left(1 - D\right)} \left(- \frac{A}{2} + \frac{A t}{T \left(1 - D\right)}\right)^{2}\, dt}}{\sqrt{T}}\\
\Delta^B_{rms}(A,B,D,T) = \frac{A}{2 \sqrt{3}}\\
\Delta^B_{avg}(A,B,D,T) = \frac{\int\limits_{0}^{D T} \left(- \frac{A}{2} + \frac{A t}{D T}\right)\, dt + \int\limits_{0}^{T \left(1 - D\right)} \left(- \frac{A}{2} + \frac{A t}{T \left(1 - D\right)}\right)\, dt}{T}\\
\Delta^B_{avg}(A,B,D,T) = 0\\
\end{align}

Elevated Right Triangle $\Delta^R$ 

B = Tri Y Midpoint 

A = triangle height 

DT = time of triangle peak
\begin{align}
\Delta^R_{rms}(A,B,D,T) = \frac{\sqrt{\int\limits_{0}^{D T} \left(- \frac{A}{2} + \frac{A t}{D T} + B\right)^{2}\, dt}}{\sqrt{T}}\\
\Delta^R_{rms}(A,B,D,T) = \frac{\sqrt{D} \sqrt{A^{2} + 12 B^{2}}}{2 \sqrt{3}}\\
\Delta^R_{avg}(A,B,D,T) = \frac{\int\limits_{0}^{D T} \left(- \frac{A}{2} + \frac{A t}{D T} + B\right)\, dt}{T}\\
\Delta^R_{avg}(A,B,D,T) = B D\\
\end{align}

Inductor rms simple
\begin{align}
I_{ref,rms} = \frac{\sqrt{\int\limits_{0}^{\pi} \frac{P_{o}^{2}}{V_{pk}^{2}}\, d\theta}}{\sqrt{\pi}}\\
I_{ref,rms} = \frac{P_{o}}{V_{pk}}\\
I_{L,rms} = I_{ref,rms}\\
\end{align}

Inductor rms with ripple
\begin{align}
\Delta i_{L,pp}(\theta) = v_{In}(\theta)\frac{\delta_{Q}(\theta)}{Lf}\\
\Delta i_{L,pp}(\theta) = \frac{V_{pk} \left(1 - \frac{V_{pk}}{V_{o}}\right)}{L f}\\
\Delta i_{L,rms,t}(\theta) = \Delta^B_{rms}(A=i_{LR,pp})\\
\Delta i_{L,rms,t}(\theta) = \frac{V_{pk} \left|{V_{o} - V_{pk}}\right|}{2 \sqrt{3} L V_{o} f}\\
\Delta I_{L,rms} = \frac{\sqrt{\int\limits_{0}^{\pi} \frac{V_{pk}^{2} \left(V_{o} - V_{pk}\right)^{2}}{12 L^{2} V_{o}^{2} f^{2}}\, d\theta}}{\sqrt{\pi}}\\
\Delta I_{L,rms} = \frac{V_{pk} \left|{V_{o} - V_{pk}}\right|}{2 \sqrt{3} L V_{o} f}\\
I_{L,rms} = \sqrt{I_{ref,rms}^2 + \Delta I_{L,rms}^2}\\
I_{L,rms} = \frac{\sqrt{12 L^{2} P_{o}^{2} V_{o}^{2} f^{2} + V_{o}^{2} V_{pk}^{4} - 2 V_{o} V_{pk}^{5} + V_{pk}^{6}}}{2 \sqrt{3} L V_{o} V_{pk} f}\\
\end{align}

Bridge rms simple
\begin{align}
I_{B,rms} = I_{L,rms}\\
I_{B,rms} = \frac{P_{o}}{V_{pk}}\\
\end{align}

Bridge rms with ripple
\begin{align}
I_{B,rms} = I_{L,rms}\\
I_{B,rms} = \frac{\sqrt{12 L^{2} P_{o}^{2} V_{o}^{2} f^{2} + V_{o}^{2} V_{pk}^{4} - 2 V_{o} V_{pk}^{5} + V_{pk}^{6}}}{2 \sqrt{3} L V_{o} V_{pk} f}\\
\end{align}

Bridge avg
\begin{align}
I_{B,avg} = \frac{\int\limits_{0}^{\pi} \frac{P_{o}}{V_{pk}}\, d\theta}{\pi}\\
I_{B,avg} = \frac{P_{o}}{V_{pk}}\\
\end{align}

Switch rms simple
\begin{align}
i_{Q,rms,t}(\theta) = \Delta^R_{rms} \big(B=i_{ref}, A=0, D=\delta_{Q} \big)\\
i_{Q,rms,t}(\theta) = \frac{P_{o} \sqrt{V_{o} - V_{pk}}}{\sqrt{V_{o}} V_{pk}}\\
I_{Q,rms} = \frac{\sqrt{\int\limits_{0}^{\pi} \frac{P_{o}^{2} \left(V_{o} - V_{pk}\right)}{V_{o} V_{pk}^{2}}\, d\theta}}{\sqrt{\pi}}\\
I_{Q,rms} = \frac{P_{o} \sqrt{V_{o} - V_{pk}}}{\sqrt{V_{o}} V_{pk}}\\
\end{align}

Switch rms with ripple
\begin{align}
i_{Q,rms,t}(\theta) = \Delta^R_{rms} \big(B=i_{ref},A=i_{LR,pp},D=\delta_{Q} \big)\\
\text{\scalebox{0.75}{$i_{Q,rms,t}(\theta) = \frac{\sqrt{\left(V_{o} - V_{pk}\right) \left(12 L^{2} P_{o}^{2} V_{o}^{2} f^{2} + V_{o}^{2} V_{pk}^{4} - 2 V_{o} V_{pk}^{5} + V_{pk}^{6}\right)}}{2 \sqrt{3} L V_{o}^{\frac{3}{2}} V_{pk} f}$}}\\
I_{Q,rms} = \frac{\sqrt{\int\limits_{0}^{\pi} \frac{\left(V_{o} - V_{pk}\right) \left(12 L^{2} P_{o}^{2} V_{o}^{2} f^{2} + V_{o}^{2} V_{pk}^{4} - 2 V_{o} V_{pk}^{5} + V_{pk}^{6}\right)}{12 L^{2} V_{o}^{3} V_{pk}^{2} f^{2}}\, d\theta}}{\sqrt{\pi}}\\
\text{\scalebox{0.75}{$I_{Q,rms} = \frac{\sqrt{\left(V_{o} - V_{pk}\right) \left(12 L^{2} P_{o}^{2} V_{o}^{2} f^{2} + V_{o}^{2} V_{pk}^{4} - 2 V_{o} V_{pk}^{5} + V_{pk}^{6}\right)}}{2 \sqrt{3} L V_{o}^{\frac{3}{2}} V_{pk} f}$}}\\
\end{align}

Switch avg
\begin{align}
i_{Q,avg,t}(\theta) = \Delta^R_{avg} \big(B=i_{ref}, D=\delta_{Q} \big)\\
I_{Q,avg,t} = \frac{P_{o} \left|{V_{o} - V_{pk}}\right|}{V_{o} V_{pk}}\\
I_{Q,avg} = \frac{\int\limits_{0}^{\pi} \frac{P_{o} \left(1 - \frac{V_{pk}}{V_{o}}\right)}{V_{pk}}\, d\theta}{\pi}\\
I_{Q,avg} = \frac{P_{o} \left|{V_{o} - V_{pk}}\right|}{V_{o} V_{pk}}\\
\end{align}

Switch switching loss timings
\begin{align}
t_{IR} = t_{2} - t_{1} = R_{g}C_{iss,test}\text{ln}\bigg(\frac{V_{gs,max}-V_{th}}{V_{gs,max}-V_{gp}}\bigg)\\
t_{VF} = t_{3} = \frac{R_{g}Q_{gd,test}V_{ds,max}}{V_{ds,test}(V_{gs,max} - V_{gp})}\\
t_{VR} = t_{5} = \frac{R_{g}Q_{gd,test}V_{ds,max}}{V_{ds,test}V_{gp}}\\
t_{IF} = t_{6} = R_{g}C_{iss,test}\text{ln}\bigg(\frac{V_{gp}}{V_{th}}\bigg)\\
t_{ON} = t_{IR} + t_{VF}\\
t_{OFF} = t_{IF} + t_{VR}\\
\end{align}

Switch switching loss simple
\begin{align}
P_{Q,sw,t}(\theta) = \frac{V_{o}f}{2}I_{ref}(\theta)(t_{ON} + t_{OFF})\\
P_{Q,sw,t}(\theta) = \frac{P_{o} V_{o} f \left(T_{OFF} + T_{ON}\right)}{2 V_{pk}}\\
P_{Q,sw} = \frac{\int\limits_{0}^{\pi} \frac{P_{o} V_{o} f \left(T_{OFF} + T_{ON}\right)}{2 V_{pk}}\, d\theta}{\pi}\\
P_{Q,sw} = \frac{P_{o} V_{o} f \left(T_{OFF} + T_{ON}\right)}{2 V_{pk}}\\
\end{align}

Switch switching loss with ripple
\begin{align}
P_{Q,sw,t}(\theta) = \frac{V_{o}f}{2}\bigg(\big(I_{ref}(\theta)-\Delta i_{L,pp}(\theta)\big)t_{ON} + \big(I_{ref}(\theta)+\Delta i_{L,pp}(\theta)\big)t_{OFF}\bigg)\\
\text{\scalebox{0.75}{$P_{Q,sw,t}(\theta) = \frac{V_{o} f \left(T_{OFF} \left(\frac{P_{o}}{V_{pk}} + \frac{V_{pk} \left(1 - \frac{V_{pk}}{V_{o}}\right)}{2 L f}\right) + T_{ON} \left(\frac{P_{o}}{V_{pk}} - \frac{V_{pk} \left(1 - \frac{V_{pk}}{V_{o}}\right)}{2 L f}\right)\right)}{2}$}}\\
P_{Q,sw} = \frac{\int\limits_{0}^{\pi} \frac{V_{o} f \left(T_{OFF} \left(\frac{P_{o}}{V_{pk}} + \frac{V_{pk} \left(1 - \frac{V_{pk}}{V_{o}}\right)}{2 L f}\right) + T_{ON} \left(\frac{P_{o}}{V_{pk}} - \frac{V_{pk} \left(1 - \frac{V_{pk}}{V_{o}}\right)}{2 L f}\right)\right)}{2}\, d\theta}{\pi}\\
\text{\scalebox{0.6}{$P_{Q,sw} = \frac{\left|{2 L P_{o} T_{OFF} V_{o} f + 2 L P_{o} T_{ON} V_{o} f + T_{OFF} V_{o} V_{pk}^{2} - T_{OFF} V_{pk}^{3} - T_{ON} V_{o} V_{pk}^{2} + T_{ON} V_{pk}^{3}}\right|}{4 L V_{pk}}$}}\\
\end{align}

Switch switching loss output capacitance
\begin{align}
P_{Q,sw,c}(\theta) = \frac{C_{oss} V_{o}^{2} f}{2}\\
P_{Q,sw,c} = \frac{\int\limits_{0}^{\pi} \frac{C_{oss} V_{o}^{2} f}{2}\, d\theta}{\pi}\\
P_{Q,sw,c} = \frac{C_{oss} V_{o}^{2} f}{2}\\
\end{align}

Boost Diode simple
\begin{align}
i_{D,rms,t}(\theta) = \Delta^R_{rms} \big(B=i_{ref}, A=0, D=\delta_{D} \big)\\
i_{D,rms,t}(\theta) = \frac{P_{o}}{\sqrt{V_{o}} \sqrt{V_{pk}}}\\
I_{D,rms} = \frac{\sqrt{\int\limits_{0}^{\pi} \frac{P_{o}^{2}}{V_{o} V_{pk}}\, d\theta}}{\sqrt{\pi}}\\
I_{D,rms} = \frac{P_{o}}{\sqrt{V_{o}} \sqrt{V_{pk}}}\\
\end{align}

Boost Diode with ripple
\begin{align}
i_{D,rms,t}(\theta) = \Delta^R_{rms} \big(B=i_{ref},A=i_{LR,pp},D=\delta_{D} \big)\\
\text{\scalebox{0.75}{$i_{D,rms,t}(\theta) = \frac{\sqrt{12 L^{2} P_{o}^{2} V_{o}^{2} f^{2} + V_{o}^{2} V_{pk}^{4} - 2 V_{o} V_{pk}^{5} + V_{pk}^{6}}}{2 \sqrt{3} L V_{o}^{\frac{3}{2}} \sqrt{V_{pk}} f}$}}\\
I_{D,rms} = \frac{\sqrt{\int\limits_{0}^{\pi} \frac{12 L^{2} P_{o}^{2} V_{o}^{2} f^{2} + V_{o}^{2} V_{pk}^{4} - 2 V_{o} V_{pk}^{5} + V_{pk}^{6}}{12 L^{2} V_{o}^{3} V_{pk} f^{2}}\, d\theta}}{\sqrt{\pi}}\\
I_{D,rms} = \frac{\sqrt{12 L^{2} P_{o}^{2} V_{o}^{2} f^{2} + V_{o}^{2} V_{pk}^{4} - 2 V_{o} V_{pk}^{5} + V_{pk}^{6}}}{2 \sqrt{3} L V_{o}^{\frac{3}{2}} \sqrt{V_{pk}} f}\\
\end{align}

Boost Diode avg
\begin{align}
i_{D,avg,t}(\theta) = \Delta^R_{avg} \big(B=i_{ref}, D=\delta_{D} \big)\\
I_{D,avg,t} = \frac{P_{o}}{V_{o}}\\
I_{D,avg} = \frac{\int\limits_{0}^{\pi} \frac{P_{o}}{V_{o}}\, d\theta}{\pi}\\
I_{D,avg} = \frac{P_{o}}{V_{o}}\\
\end{align}

Boost Diode switching loss timings
\begin{align}
K_{Q} = \frac{I_{rr,0}T_{rr,0}}{2\sqrt{I_{F,0}}}\\
S = \frac{T_{rr,0}\frac{dI_{D,0}}{dt}}{I_{rr,0}} - 1\\
I_{rr} = \sqrt{\frac{2\frac{dI_{D}}{dt}K_{Q}\sqrt{I_{F}}}{1+S}}\\
T_{a} = \frac{I_{rr}}{\frac{dI_{D}}{dt}}\\
T_{b} = ST_{a}\\
E_{Q} = V_{DS}\big(\frac{I_{rr}}{2}T_{a}+\frac{I_{rr}}{4}T_{b}\big)\\
E_{D} = \frac{V_{R}I_{rr}}{4}T_{b}\\
\end{align}

Boost Diode switching loss reverse recovery simple
\begin{align}
I_{F} = \frac{P_{o}}{V_{pk}}\\
\frac{dI_{D}}{dt} = \frac{P_{o}}{T_{IR} V_{pk}}\\
I_{rr} = \frac{\sqrt{2} \sqrt{K_{Q}} P_{o}^{\frac{3}{4}}}{\sqrt{T_{IR}} V_{pk}^{\frac{3}{4}} \sqrt{S + 1}}\\
T_{a} = \frac{\sqrt{2} \sqrt{K_{Q}} \sqrt{T_{IR}} \sqrt[4]{V_{pk}}}{\sqrt[4]{P_{o}} \sqrt{S + 1}}\\
T_{b} = \frac{\sqrt{2} \sqrt{K_{Q}} S \sqrt{T_{IR}} \sqrt[4]{V_{pk}}}{\sqrt[4]{P_{o}} \sqrt{S + 1}}\\
E_{Qrr} = \frac{K_{Q} \sqrt{P_{o}} V_{o} \left(S + 2\right)}{2 \sqrt{V_{pk}} \left(S + 1\right)}\\
E_{Drr} = \frac{K_{Q} \sqrt{P_{o}} S V_{o}}{2 \sqrt{V_{pk}} \left(S + 1\right)}\\
P_{D,sw,rr}(\theta) = \frac{K_{Q} \sqrt{P_{o}} V_{o} f}{\sqrt{V_{pk}}}\\
P_{D,sw,rr} = \frac{\int\limits_{0}^{\pi} \frac{K_{Q} \sqrt{P_{o}} V_{o} f}{\sqrt{V_{pk}}}\, d\theta}{\pi}\\
P_{D,sw,rr} = \frac{K_{Q} \sqrt{P_{o}} V_{o} f}{\sqrt{V_{pk}}}\\
\end{align}

Boost Diode switching loss reverse recovery with ripple
\begin{align}
I_{F} = \frac{P_{o}}{V_{pk}} - \frac{V_{pk} \left(1 - \frac{V_{pk}}{V_{o}}\right)}{2 L f}\\
\frac{dI_{D}}{dt} = \frac{\frac{P_{o}}{V_{pk}} - \frac{V_{pk} \left(1 - \frac{V_{pk}}{V_{o}}\right)}{2 L f}}{T_{IR}}\\
I_{rr} = \frac{\sqrt{2} \sqrt{K_{Q}} \sqrt{\left(\frac{P_{o}}{V_{pk}} - \frac{V_{pk} \left(1 - \frac{V_{pk}}{V_{o}}\right)}{2 L f}\right)^{\frac{3}{2}}}}{\sqrt{T_{IR}} \sqrt{S + 1}}\\
T_{a} = \frac{\sqrt{2} \sqrt{K_{Q}} \sqrt{T_{IR}} \sqrt{\left(\frac{P_{o}}{V_{pk}} - \frac{V_{pk} \left(1 - \frac{V_{pk}}{V_{o}}\right)}{2 L f}\right)^{\frac{3}{2}}}}{\sqrt{S + 1} \left(\frac{P_{o}}{V_{pk}} - \frac{V_{pk} \left(1 - \frac{V_{pk}}{V_{o}}\right)}{2 L f}\right)}\\
T_{b} = \frac{\sqrt{2} \sqrt{K_{Q}} S \sqrt{T_{IR}} \sqrt{\left(\frac{P_{o}}{V_{pk}} - \frac{V_{pk} \left(1 - \frac{V_{pk}}{V_{o}}\right)}{2 L f}\right)^{\frac{3}{2}}}}{\sqrt{S + 1} \left(\frac{P_{o}}{V_{pk}} - \frac{V_{pk} \left(1 - \frac{V_{pk}}{V_{o}}\right)}{2 L f}\right)}\\
E_{Qrr} = \frac{\sqrt{2} K_{Q} \sqrt{V_{o}} \left(S + 2\right) \sqrt{2 L P_{o} V_{o} f - V_{pk}^{2} \left(V_{o} - V_{pk}\right)}}{4 \sqrt{L} \sqrt{V_{pk}} \sqrt{f} \left(S + 1\right)}\\
E_{Drr} = \frac{K_{Q} S V_{o} \sqrt{\frac{P_{o}}{V_{pk}} - \frac{V_{pk} \left(1 - \frac{V_{pk}}{V_{o}}\right)}{2 L f}}}{2 \left(S + 1\right)}\\
\end{align}


\begin{align}
P_{D,sw,rr}(\theta) = \frac{\sqrt{2} K_{Q} \sqrt{V_{o}} \sqrt{f} \sqrt{2 L P_{o} V_{o} f - V_{pk}^{2} \left(V_{o} - V_{pk}\right)}}{2 \sqrt{L} \sqrt{V_{pk}}}\\
P_{D,sw,rr} = \frac{\int\limits_{0}^{\pi} \frac{\sqrt{2} K_{Q} \sqrt{V_{o}} \sqrt{f} \sqrt{2 L P_{o} V_{o} f - V_{pk}^{2} \left(V_{o} - V_{pk}\right)}}{2 \sqrt{L} \sqrt{V_{pk}}}\, d\theta}{\pi}\\
P_{D,sw,rr} = \frac{K_{Q} \sqrt{V_{o}} \sqrt{f} \sqrt{2 L P_{o} V_{o} f - V_{o} V_{pk}^{2} + V_{pk}^{3}}}{\sqrt{2} \sqrt{L} \sqrt{V_{pk}}}\\
\end{align}

Boost Diode switching loss junction capacitance
\begin{align}
P_{D,sw,c}(\theta) = \frac{C_{j}V_{D,bl}^{2}(\theta)f}{2}\\
P_{D,sw,c}(\theta) = \frac{C_{j} V_{o}^{2} f}{2}\\
P_{D,sw,c} = \frac{\int\limits_{0}^{\pi} \frac{C_{j} V_{o}^{2} f}{2}\, d\theta}{\pi}\\
P_{D,sw,c} = \frac{C_{j} V_{o}^{2} f}{2}\\
\end{align}

Cap rms simple
\begin{align}
I_{C,rms} = \sqrt{I_{D,rms}^2 - (\frac{P_o}{V_o})^2}\\
I_{C,rms} = \frac{P_{o} \sqrt{V_{o} - V_{pk}}}{V_{o} \sqrt{V_{pk}}}\\
\end{align}

Cap rms with ripple
\begin{align}
I_{C,rms} = \sqrt{I_{D,rms}^2 - (\frac{P_o}{V_o})^2}\\
I_{C,rms} = \frac{\sqrt{\left(V_{o} - V_{pk}\right) \left(12 L^{2} P_{o}^{2} V_{o} f^{2} + V_{o} V_{pk}^{4} - V_{pk}^{5}\right)}}{2 \sqrt{3} L V_{o}^{\frac{3}{2}} \sqrt{V_{pk}} f}\\
\end{align}
\end{document}
